theories/DSubSyn/lr/unary_lr.v
@@ -227,24 +227,24 @@ Section logrel_part2.
   Global Arguments ietp /.
   Notation "Γ ⊨ e : T" := (ietp Γ T e) (at level 74, e, T at next level).
 
-  Definition step_indexed_ietp Γ T e i: iProp Σ :=
+  Definition ietpi Γ T e i: iProp Σ :=
     (□∀ ρ, ⟦Γ⟧* ρ → ▷^i ⟦T⟧ₑ ρ (e.|[ρ]))%I.
-  Global Arguments step_indexed_ietp /.
-  Notation "Γ ⊨ e : T , i" := (step_indexed_ietp Γ T e i) (at level 74, e, T at next level).
+  Global Arguments ietpi /.
+  Notation "Γ ⊨ e : T , i" := (ietpi Γ T e i) (at level 74, e, T at next level).
 
   (** Indexed Subtyping. Defined on closed values. We must require closedness
       explicitly, since closedness now does not follow from being well-typed later. *)
-  Definition step_indexed_ivstp Γ T1 T2 i j: iProp Σ :=
+  Definition istpi Γ T1 T2 i j: iProp Σ :=
     (□∀ ρ v, ⟦Γ⟧* ρ → (▷^i ⟦T1⟧ ρ v) → ▷^j ⟦T2⟧ ρ v)%I.
-  Global Arguments step_indexed_ivstp /.
+  Global Arguments istpi /.
 
   Definition delayed_ivstp Γ T1 T2 i: iProp Σ :=
     (□ ∀ ρ, ⟦Γ⟧*ρ → ▷^i ∀v, ⟦T1⟧ ρ v → ⟦T2⟧ ρ v)%I.
   Global Arguments delayed_ivstp /.
 
   Global Instance ietp_persistent Γ T e : Persistent (ietp Γ T e) := _.
-  Global Instance step_indexed_ietp_persistent Γ T e i : Persistent (step_indexed_ietp Γ T e i) := _.
-  Global Instance step_indexed_ivstp_persistent Γ T1 T2 i j : Persistent (step_indexed_ivstp Γ T1 T2 i j) := _.
+  Global Instance ietpi_persistent Γ T e i : Persistent (ietpi Γ T e i) := _.
+  Global Instance istpi_persistent Γ T1 T2 i j : Persistent (istpi Γ T1 T2 i j) := _.
 End logrel_part2.
 
 Notation "⟦ Γ ⟧*" := (interp_env Γ).
@@ -252,9 +252,9 @@ Notation "⟦ Γ ⟧*" := (interp_env Γ).
 (** Expression typing *)
 Notation "Γ ⊨ e : T" := (ietp Γ T e) (at level 74, e, T at next level).
 (** Indexed expression typing *)
-Notation "Γ ⊨ e : T , i" := (step_indexed_ietp Γ T e i) (at level 74, e, T at next level).
+Notation "Γ ⊨ e : T , i" := (ietpi Γ T e i) (at level 74, e, T at next level).
 
-Notation "Γ ⊨ T1 , i <: T2 , j " := (step_indexed_ivstp Γ T1 T2 i j) (at level 74, T1, T2, i, j at next level).
+Notation "Γ ⊨ T1 , i <: T2 , j " := (istpi Γ T1 T2 i j) (at level 74, T1, T2, i, j at next level).
 Notation "Γ ⊨[ i  ] T1 <: T2" := (delayed_ivstp Γ T1 T2 i) (at level 74, T1, T2 at next level).
 
 Section logrel_lemmas.
